PropositionalLogic/ClassicalPropositionalLogic.v
@@ -1,4 +1,5 @@
 Require Import Logic.LogicBase.
+Require Import Logic.SyntacticReduction.
 Require Import Logic.PropositionalLogic.Syntax.
 
 Local Open Scope logic_base.
@@ -6,19 +7,21 @@ Local Open Scope PropositionalLogic.
 
 Definition reduce {L: Language} {nL: NormalLanguage L} {pL: PropositionalLanguage L}: relation expr:=
   clos_refl_trans _
-   (prop_congr
+   (propag_reduce
      (relation_disjunction
         ImpNegAsPrime.atomic_reduce
         (relation_disjunction
           ReduceIff.atomic_reduce
-          ReduceTrueFalse.atomic_reduce))).
+          ReduceFalse.atomic_reduce))).
 
 Class ClassicalPropositionalLogic (L: Language) {nL: NormalLanguage L} {pL: PropositionalLanguage L} (Gamma: ProofTheory L) := {
-  syntactic_reduction_rule: forall x y, reduce x y -> |-- x -> |-- y;
+  syntactic_reduction_rule1: forall x y, reduce x y -> |-- x -> |-- y;
+  syntactic_reduction_rule2: forall x y, reduce x y -> |-- y -> |-- x;
   modus_ponens: forall x y, |-- (x --> y) -> |-- x -> |-- y;
   axiom1: forall x y, |-- (x --> (y --> x));
   axiom2: forall x y z, |-- ((x --> y --> z) --> (x --> y) --> (x --> z));
-  axiom3: forall x y, |-- ((~~ y --> x) --> (~~ y --> ~~ x) --> y)
+  axiom3: forall x y, |-- ((~~ y --> x) --> (~~ y --> ~~ x) --> y);
+  true_provable: provable TT
 }.
 
 Lemma imp_refl: forall (L: Language) {nL: NormalLanguage L} {pL: PropositionalLanguage L} {Gamma: ProofTheory L} {cpGamma: ClassicalPropositionalLogic L Gamma} (x: expr), |-- x --> x.
@@ -55,11 +58,13 @@ Section ClassicalPropositionalLogic.
 Context (Var: Type).
 
 Inductive provable: @expr (PropositionalLanguage.L Var) -> Prop :=
-| syntactic_reduction_rule: forall x y, reduce x y -> provable x -> provable y
+| syntactic_reduction_rule1: forall x y, reduce x y -> provable x -> provable y
+| syntactic_reduction_rule2: forall x y, reduce x y -> provable y -> provable x
 | modus_ponens: forall x y, provable (x --> y) -> provable x -> provable y
 | axiom1: forall x y, provable (x --> (y --> x))
 | axiom2: forall x y z, provable ((x --> y --> z) --> (x --> y) --> (x --> z))
-| axiom3: forall x y, provable ((~~ y --> x) --> (~~ y --> ~~ x) --> y).
+| axiom3: forall x y, provable ((~~ y --> x) --> (~~ y --> ~~ x) --> y)
+| true_provable: provable TT.
 (* Elliott Mendelson, Introduction to Mathematical Logic, Second Edition (New York: D. Van Nostrand, 1979) *)
 
 Instance AG: AxiomaticProofTheory.AxiomaticProofTheory (PropositionalLanguage.L Var) :=
@@ -70,11 +75,13 @@ Instance G: ProofTheory (PropositionalLanguage.L Var) := AxiomaticProofTheory.G 
 Instance cpG: ClassicalPropositionalLogic (PropositionalLanguage.L Var) G.
 Proof.
   constructor.
-  + apply syntactic_reduction_rule.
+  + apply syntactic_reduction_rule1.
+  + apply syntactic_reduction_rule2.
   + apply modus_ponens.
   + apply axiom1.
   + apply axiom2.
   + apply axiom3.
+  + apply true_provable.
 Qed.
 
 End ClassicalPropositionalLogic.
