PropositionalLogic/Syntax.v
@@ -1,39 +1,37 @@
-Require Export Coq.Relations.Relation_Definitions.
-Require Export Coq.Relations.Relation_Operators.
-Require Export Coq.Relations.Relation_Definitions.
-Require Export Coq.Classes.RelationClasses.
 Require Import Logic.LogicBase.
+Require Import Logic.SyntacticReduction.
 
 Class PropositionalLanguage (L: Language) {nL: NormalLanguage L}: Type := {
   andp : expr -> expr -> expr;
   orp : expr -> expr -> expr;
   iffp : expr -> expr -> expr;
   negp : expr -> expr;
-  truep : expr
+  truep : expr;
+  and1_propag: expr -> single_propagation;
+  and2_propag: expr -> single_propagation;
+  or1_propag: expr -> single_propagation;
+  or2_propag: expr -> single_propagation;
+  iff1_propag: expr -> single_propagation;
+  iff2_propag: expr -> single_propagation;
+  neg_propag: single_propagation;
+  and1_propag_denote: forall x y, single_propagation_denote (and1_propag x) y = andp y x;
+  and2_propag_denote: forall x y, single_propagation_denote (and2_propag x) y = andp x y;
+  or1_propag_denote: forall x y, single_propagation_denote (or1_propag x) y = orp y x;
+  or2_propag_denote: forall x y, single_propagation_denote (or2_propag x) y = orp x y;
+  iff1_propag_denote: forall x y, single_propagation_denote (iff1_propag x) y = iffp y x;
+  iff2_propag_denote: forall x y, single_propagation_denote (iff2_propag x) y = iffp x y;
+  neg_propag_denote: forall x, single_propagation_denote neg_propag x = negp x
 }.
 
 Notation "x && y" := (andp x y) (at level 40, left associativity) : PropositionalLogic.
 Notation "x || y" := (orp x y) (at level 50, left associativity) : PropositionalLogic.
-Notation "x --> y" := (imp x y) (at level 55, right associativity) : PropositionalLogic.
+Notation "x --> y" := (impp x y) (at level 55, right associativity) : PropositionalLogic.
 Notation "x <--> y" := (iffp x y) (at level 60, no associativity) : PropositionalLogic.
 Notation "~~ x" := (negp x) (at level 35) : PropositionalLogic.
 Notation "'FF'" := falsep : PropositionalLogic.
 Notation "'TT'" := truep : PropositionalLogic.
 
 Local Open Scope PropositionalLogic.
-
-Inductive prop_congr {L: Language} {nL: NormalLanguage L} {pL: PropositionalLanguage L} {atomic_reduce: relation expr}: relation expr :=
-| atomic_step: forall x y, atomic_reduce x y -> prop_congr x y
-| andp_congr: forall x1 x2 y1 y2, prop_congr x1 y1 -> prop_congr x2 y2 -> prop_congr (x1 && x2) (y1 && y2)
-| orp_congr: forall x1 x2 y1 y2, prop_congr x1 y1 -> prop_congr x2 y2 -> prop_congr (x1 || x2) (y1 || y2)
-| imp_congr: forall x1 x2 y1 y2, prop_congr x1 y1 -> prop_congr x2 y2 -> prop_congr (x1 --> x2) (y1 --> y2)
-| iffp_congr: forall x1 x2 y1 y2, prop_congr x1 y1 -> prop_congr x2 y2 -> prop_congr (x1 <--> x2) (y1 <--> y2)
-| negp_congr: forall x y, prop_congr x y -> prop_congr (~~ x) (~~ y)
-.
-
-(* Locate clos_refl_trans. *)
-
-Arguments prop_congr {L} {nL} {pL} atomic_reduce _ _.
 
 Module ImpNegAsPrime.
 
@@ -59,20 +57,19 @@ Inductive atomic_reduce {L: Language} {nL: NormalLanguage L} {pL: PropositionalL
 
 End ReduceIff.
 
-Module ReduceTrueFalse.
+Module ReduceFalse.
 
 Inductive atomic_reduce {L: Language} {nL: NormalLanguage L} {pL: PropositionalLanguage L}: expr -> expr -> Prop :=
-| falsep_reduce: atomic_reduce FF (~~ TT)
-| truep_reduce: forall x, atomic_reduce TT (x --> x).
+| falsep_reduce: atomic_reduce FF (~~ TT).
 
-End ReduceTrueFalse.
+End ReduceFalse.
 
 Module PropositionalLanguage.
 
 Inductive expr {Var: Type}: Type :=
   | andp : expr -> expr -> expr
   | orp : expr -> expr -> expr
-  | imp : expr -> expr -> expr
+  | impp : expr -> expr -> expr
   | iffp : expr -> expr -> expr
   | negp : expr -> expr
   | truep : expr
@@ -81,9 +78,139 @@ Inductive expr {Var: Type}: Type :=
 
 Implicit Arguments expr.
 
-Instance L (Var: Type): Language := Build_Language (expr Var).
-Instance nL (Var: Type): NormalLanguage (L Var) := Build_NormalLanguage (L Var) falsep imp.
-Instance pL (Var: Type): PropositionalLanguage (L Var) := Build_PropositionalLanguage (L Var) (nL Var) andp orp iffp negp truep.
+Inductive single_propagation {Var: Type}: Type :=
+  | and1_propag : expr Var -> single_propagation
+  | and2_propag : expr Var -> single_propagation
+  | or1_propag : expr Var -> single_propagation
+  | or2_propag : expr Var -> single_propagation
+  | imp1_propag : expr Var -> single_propagation
+  | imp2_propag : expr Var -> single_propagation
+  | iff1_propag : expr Var -> single_propagation
+  | iff2_propag : expr Var -> single_propagation
+  | neg_propag : single_propagation
+.
+
+Implicit Arguments single_propagation.
+
+Definition single_propagation_denote {Var: Type} (sp: single_propagation Var) (x: expr Var): expr Var :=
+  match sp with
+  | and1_propag y => andp x y
+  | and2_propag y => andp y x
+  | or1_propag y => orp x y
+  | or2_propag y => orp y x
+  | imp1_propag y => impp x y
+  | imp2_propag y => impp y x
+  | iff1_propag y => iffp x y
+  | iff2_propag y => iffp y x
+  | neg_propag => negp x
+  end.
+
+Instance L (Var: Type): Language :=
+  Build_Language (expr Var) (single_propagation Var) single_propagation_denote.
+
+Instance nL (Var: Type): NormalLanguage (L Var) :=
+  Build_NormalLanguage (L Var) falsep impp imp1_propag imp2_propag (fun _ _ => eq_refl) (fun _ _ => eq_refl).
+
+Instance pL (Var: Type): PropositionalLanguage (L Var) :=
+  Build_PropositionalLanguage (L Var) (nL Var) andp orp iffp negp truep
+    and1_propag and2_propag or1_propag or2_propag iff1_propag iff2_propag neg_propag
+    (fun _ _ => eq_refl) (fun _ _ => eq_refl) (fun _ _ => eq_refl) (fun _ _ => eq_refl)
+    (fun _ _ => eq_refl) (fun _ _ => eq_refl) (fun _ => eq_refl).
+
+(*
+
+Definition mendelson_andp {Var: Type} (x y: expr Var): expr Var := negp (impp x (negp y)).
+
+Definition mendelson_orp {Var: Type} (x y: expr Var): expr Var := impp (negp x) y.
+
+Definition mendelson_iffp {Var: Type} (x y: expr Var): expr Var := mendelson_andp (impp x y) (impp y x).
+
+Fixpoint mendelson_reduce {Var: Type} (x: expr Var): expr Var :=
+  match x with
+  | andp y z => mendelson_andp (mendelson_reduce y) (mendelson_reduce z)
+  | orp y z => mendelson_orp (mendelson_reduce y) (mendelson_reduce z)
+  | impp y z => impp (mendelson_reduce y) (mendelson_reduce z)
+  | iffp y z => mendelson_iffp (mendelson_reduce y) (mendelson_reduce z)
+  | negp y => negp (mendelson_reduce y)
+  | truep => truep
+  | falsep => negp truep
+  | varp p => varp p
+  end.
+
+Fixpoint mendelson_normal_form {Var: Type} (x: expr Var): Prop :=
+  match x with
+  | andp y z => False
+  | orp y z => False
+  | impp y z => mendelson_normal_form y /\ mendelson_normal_form z
+  | iffp y z => False
+  | negp y => mendelson_normal_form y
+  | truep => True
+  | falsep => False
+  | varp p => True
+  end.
+*)
+Definition MendelsonReduction {Var: Type}: SyntacticReduction (L Var).
+  refine (Build_SyntacticReduction _
+            (relation_disjunction
+               ImpNegAsPrime.atomic_reduce
+               (relation_disjunction
+                 ReduceIff.atomic_reduce
+                 ReduceFalse.atomic_reduce))).
+(*
+            mendelson_normal_form
+            _
+            mendelson_reduce
+            _ _ _ _).
+  + simpl; intros.
+    induction x; simpl.
+    - split; [intros [] | intros HH; apply HH; clear HH].
+      clear.
+      eexists.
+      eapply (@propag_reduce_spec (L Var) _ (andp x1 x2) _ nil).
+      left; apply (@ImpNegAsPrime.andp_reduce (L Var)); auto.
+    - split; [intros [] | intros HH; apply HH; clear HH].
+      clear.
+      eexists.
+      eapply (@propag_reduce_spec (L Var) _ (orp x1 x2) _ nil).
+      left; apply (@ImpNegAsPrime.orp_reduce (L Var)); auto.
+    - split; intros.
+      * destruct H; rewrite IHx1 in H; rewrite IHx2 in H0; clear - H H0.
+        intros [y ?].
+        inversion H1; subst; clear H1.
+        destruct p as [? | sp p0].
+        Focus 1. {
+          simpl in H2; subst x.
+          destruct H3 as [HH | [HH | HH]]; inversion HH.
+        } Unfocus.
+        destruct sp; inversion H2; subst.
+        simpl in H2.
+        admit. admit.
+      * admit.
+    - admit.
+    - admit.
+    - admit.
+    - admit.
+    - admit.
+  + intros; induction x; simpl.
+    - eapply rt_trans.
+      Focus 1. {
+        apply rt_step.
+        eapply (@propag_reduce_spec (L Var) _ (andp x1 x2) _ nil).
+        left. apply (@ImpNegAsPrime.andp_reduce (L Var)).
+      } Unfocus.
+      simpl.
+      eapply rt_trans.
+      Focus 1. {
+        apply 
+  + intros; induction x; simpl; auto.
+  + intros.
+    destruct H as [? | [? | ?]]; inversion H; auto.
+  + intros.
+    destruct sp; simpl; f_equal; auto.
+
+*)        
+Defined.
+    
 
 End PropositionalLanguage.
 
