PropositionalLogic/Complete_Classical_Trivial.v
@@ -1,0 +1,17 @@
+Require Import Logic.LogicBase.
+Require Import Logic.PropositionalLogic.Syntax.
+Require Import Logic.PropositionalLogic.ClassicalPropositionalLogic.
+Require Import Logic.PropositionalLogic.TrivialSemantics.
+
+Local Open Scope logic_base.
+Local Open Scope PropositionalLogic.
+
+Definition MCS (Var: Type): Type := sig (maximal_consistent (ClassicalPropositionalLogic.G Var)).
+
+Definition canonical_model {Var: Type} (Phi: MCS Var): @model _ (TrivialSemantics.SM Var) :=
+  fun p => (proj1_sig Phi (PropositionalLanguage.varp p)).
+
+Lemma truth_lemma {Var: Type}: forall (Phi: MCS Var) x, canonical_model Phi |= x <-> proj1_sig Phi x.
+Proof.
+  intros.
+Abort.
