SyntacticReduction.v
@@ -1,0 +1,78 @@
+Require Import Logic.LogicBase.
+Require Export Coq.Relations.Relation_Definitions.
+Require Export Coq.Relations.Relation_Operators.
+Require Export Coq.Relations.Relation_Definitions.
+Require Export Coq.Classes.RelationClasses.
+
+Inductive propag_reduce {L: Language} (atomic_reduce: expr -> expr -> Prop): expr -> expr -> Prop :=
+  propag_reduce_spec: forall x y p, atomic_reduce x y ->
+    propag_reduce atomic_reduce (propagation_denote p x) (propagation_denote p y).
+
+Class SyntacticReduction (L: Language) : Type := {
+  atomic_reduce: expr -> expr -> Prop;
+  single_step_reduce := propag_reduce atomic_reduce;
+  reduce := clos_refl_trans _ single_step_reduce
+(*
+  normal_form: expr -> Prop;
+  normal_form_spec1: forall x, normal_form x <-> ~ exists y, single_step_reduce x y;
+  reduce_function: expr -> expr;
+  reduce_function_sound: forall x, reduce x (reduce_function x);
+  reduce_function_normal: forall x, normal_form (reduce_function x);
+  atomic_reduce_preserve_reduce_function:
+    forall x y, atomic_reduce x y -> reduce_function x = reduce_function y;
+  single_propagation_preserve_reduce_function:
+    forall x y sp, reduce_function x = reduce_function y ->
+      reduce_function (single_propagation_denote sp x) = reduce_function (single_propagation_denote sp y)
+*)
+}.
+
+(*
+Lemma single_step_reduce_preserve_reduce_function {L: Language} {SD: SyntacticReduction L}:
+  forall x y, single_step_reduce x y -> reduce_function x = reduce_function y.
+Proof.
+  intros.
+  destruct H.
+  induction p; simpl.
+  + apply atomic_reduce_preserve_reduce_function; auto.
+  + apply single_propagation_preserve_reduce_function; auto.
+Qed.
+
+Lemma reduce_preserve_reduce_function {L: Language} {SD: SyntacticReduction L}:
+  forall x y, reduce x y -> reduce_function x = reduce_function y.
+Proof.
+  intros.
+  induction H.
+  + apply single_step_reduce_preserve_reduce_function; auto.
+  + reflexivity.
+  + etransitivity; eauto.
+Qed.
+
+Lemma normal_form_spec2 {L: Language} {SD: SyntacticReduction L}:
+  forall x, normal_form x <-> reduce_function x = x.
+Proof.
+  intros.
+  split; intros.
+  + pose proof reduce_function_sound x.
+    rewrite normal_form_spec1 in H.
+    remember (reduce_function x) as y; clear Heqy.
+    induction H0.
+    - exfalso.
+      apply H; exists y; auto.
+    - auto.
+    - specialize (IHclos_refl_trans1 H).
+      subst y.
+      specialize (IHclos_refl_trans2 H).
+      auto.
+  + rewrite <- H; apply reduce_function_normal.
+Qed.
+
+Lemma reduce_unique {L: Language} {SD: SyntacticReduction L}:
+  forall x y, normal_form y -> reduce x y -> reduce_function x = y.
+Proof.
+  intros.
+  apply reduce_preserve_reduce_function in H0.
+  apply normal_form_spec2 in H.
+  congruence.
+Qed.
+
+*)
